src/Std/Data/DHashMap/Internal/List/Associative.lean
@@ -24,34 +24,34 @@ variable {α : Type u} {β : α → Type v} {γ : α → Type w}
 namespace Std.DHashMap.Internal.List
 
 @[elab_as_elim]
-theorem assoc_induction {motive : List (Σ a, β a) → Prop} (nil : motive [])
-    (cons : (k : α) → (v : β k) → (tail : List (Σ a, β a)) → motive tail → motive (⟨k, v⟩ :: tail)) :
-    (t : List (Σ a, β a)) → motive t
+theorem assoc_induction {motive : List ((a : α) × β a) → Prop} (nil : motive [])
+    (cons : (k : α) → (v : β k) → (tail : List ((a : α) × β a)) → motive tail → motive (⟨k, v⟩ :: tail)) :
+    (t : List ((a : α) × β a)) → motive t
   | [] => nil
   | ⟨_, _⟩ :: _ => cons _ _ _ (assoc_induction nil cons _)
 
-def getEntry? [BEq α] (a : α) : List (Σ a, β a) → Option (Σ a, β a)
+def getEntry? [BEq α] (a : α) : List ((a : α) × β a) → Option ((a : α) × β a)
   | [] => none
   | ⟨k, v⟩ :: l => bif a == k then some ⟨k, v⟩ else getEntry? a l
 
-@[simp] theorem getEntry?_nil [BEq α] {a : α} : getEntry? a ([] : List (Σ a, β a)) = none := rfl
-theorem getEntry?_cons [BEq α] {l : List (Σ a, β a)} {k a : α} {v : β k} :
+@[simp] theorem getEntry?_nil [BEq α] {a : α} : getEntry? a ([] : List ((a : α) × β a)) = none := rfl
+theorem getEntry?_cons [BEq α] {l : List ((a : α) × β a)} {k a : α} {v : β k} :
     getEntry? a (⟨k, v⟩ :: l) = bif a == k then some ⟨k, v⟩ else getEntry? a l := rfl
 
-theorem getEntry?_cons_of_true [BEq α] {l : List (Σ a, β a)} {k a : α} {v : β k} (h : a == k) :
+theorem getEntry?_cons_of_true [BEq α] {l : List ((a : α) × β a)} {k a : α} {v : β k} (h : a == k) :
     getEntry? a (⟨k, v⟩ :: l) = some ⟨k, v⟩ := by
   simp [getEntry?, h]
 
-theorem getEntry?_cons_of_false [BEq α] {l : List (Σ a, β a)} {k a : α} {v : β k} (h : (a == k) = false) :
+theorem getEntry?_cons_of_false [BEq α] {l : List ((a : α) × β a)} {k a : α} {v : β k} (h : (a == k) = false) :
     getEntry? a (⟨k, v⟩ :: l) = getEntry? a l := by
   simp [getEntry?, h]
 
 @[simp]
-theorem getEntry?_cons_self [BEq α] [ReflBEq α] {l : List (Σ a, β a)} {k : α} {v : β k} :
+theorem getEntry?_cons_self [BEq α] [ReflBEq α] {l : List ((a : α) × β a)} {k : α} {v : β k} :
     getEntry? k (⟨k, v⟩ :: l) = some ⟨k, v⟩ :=
   getEntry?_cons_of_true BEq.refl
 
-theorem getEntry?_eq_some [BEq α] {l : List (Σ a, β a)} {a : α} {p : Σ a, β a}
+theorem getEntry?_eq_some [BEq α] {l : List ((a : α) × β a)} {a : α} {p : (a : α) × β a}
     (h : getEntry? a l = some p) : a == p.1 := by
   induction l using assoc_induction
   · simp at h
@@ -63,7 +63,7 @@ theorem getEntry?_eq_some [BEq α] {l : List (Σ a, β a)} {a : α} {p : Σ a, �
       obtain rfl := congrArg Sigma.fst h
       exact h'
 
-theorem getEntry?_congr [BEq α] [PartialEquivBEq α] {l : List (Σ a, β a)} {a b : α} (h : a == b) :
+theorem getEntry?_congr [BEq α] [PartialEquivBEq α] {l : List ((a : α) × β a)} {a b : α} (h : a == b) :
     getEntry? a l = getEntry? b l := by
   induction l using assoc_induction
   · simp
@@ -73,7 +73,7 @@ theorem getEntry?_congr [BEq α] [PartialEquivBEq α] {l : List (Σ a, β a)} {a
       rw [getEntry?_cons_of_false h', getEntry?_cons_of_false h₂, ih]
     · rw [getEntry?_cons_of_true h', getEntry?_cons_of_true (BEq.trans h h')]
 
-theorem isEmpty_eq_false_iff_exists_isSome_getEntry? [BEq α] [ReflBEq α] : {l : List (Σ a, β a)} →
+theorem isEmpty_eq_false_iff_exists_isSome_getEntry? [BEq α] [ReflBEq α] : {l : List ((a : α) × β a)} →
     l.isEmpty = false ↔ ∃ a, (getEntry? a l).isSome
   | [] => by simp
   | (⟨k, v⟩::l) => by simpa using ⟨k, by simp⟩
@@ -122,25 +122,25 @@ theorem isEmpty_eq_false_iff_exists_isSome_getValue? [BEq α] [ReflBEq α] {l : 
 
 end
 
-def getValueCast? [BEq α] [LawfulBEq α] (a : α) : List (Σ a, β a) → Option (β a)
+def getValueCast? [BEq α] [LawfulBEq α] (a : α) : List ((a : α) × β a) → Option (β a)
   | [] => none
   | ⟨k, v⟩ :: l => if h : a == k then some (cast (congrArg β (eq_of_beq h).symm) v) else getValueCast? a l
 
 @[simp] theorem getValueCast?_nil [BEq α] [LawfulBEq α] {a : α} :
-    getValueCast? a ([] : List (Σ a, β a)) = none := rfl
-theorem getValueCast?_cons [BEq α] [LawfulBEq α] {l : List (Σ a, β a)} {k a : α} {v : β k} :
+    getValueCast? a ([] : List ((a : α) × β a)) = none := rfl
+theorem getValueCast?_cons [BEq α] [LawfulBEq α] {l : List ((a : α) × β a)} {k a : α} {v : β k} :
     getValueCast? a (⟨k, v⟩ :: l) = if h : a == k then some (cast (congrArg β (eq_of_beq h).symm) v) else getValueCast? a l := rfl
 
-theorem getValueCast?_cons_of_true [BEq α] [LawfulBEq α] {l : List (Σ a, β a)} {k a : α} {v : β k} (h : a == k) :
+theorem getValueCast?_cons_of_true [BEq α] [LawfulBEq α] {l : List ((a : α) × β a)} {k a : α} {v : β k} (h : a == k) :
     getValueCast? a (⟨k, v⟩ :: l) = some (cast (congrArg β (eq_of_beq h).symm) v) := by
   simp [getValueCast?, h]
 
-theorem getValueCast?_cons_of_false [BEq α] [LawfulBEq α] {l : List (Σ a, β a)} {k a : α} {v : β k}
+theorem getValueCast?_cons_of_false [BEq α] [LawfulBEq α] {l : List ((a : α) × β a)} {k a : α} {v : β k}
     (h : (a == k) = false) : getValueCast? a (⟨k, v⟩ :: l) = getValueCast? a l := by
   simp [getValueCast?, h]
 
 @[simp]
-theorem getValueCast?_cons_self [BEq α] [LawfulBEq α] {l : List (Σ a, β a)} {k : α} {v : β k} :
+theorem getValueCast?_cons_self [BEq α] [LawfulBEq α] {l : List ((a : α) × β a)} {k : α} {v : β k} :
     getValueCast? k (⟨k, v⟩ :: l) = some v := by
   rw [getValueCast?_cons_of_true BEq.refl, cast_eq]
 
@@ -177,7 +177,7 @@ private theorem Option.isSome_dmap {o : Option α} {f : (a : α) → (o = some a
 
 end
 
-theorem getValueCast?_eq_getEntry? [BEq α] [LawfulBEq α] {l : List (Σ a, β a)} {a : α} :
+theorem getValueCast?_eq_getEntry? [BEq α] [LawfulBEq α] {l : List ((a : α) × β a)} {a : α} :
     getValueCast? a l = Option.dmap (getEntry? a l) (fun p h => cast (congrArg β (eq_of_beq (getEntry?_eq_some h)).symm) p.2) := by
   induction l using assoc_induction
   · simp
@@ -186,47 +186,47 @@ theorem getValueCast?_eq_getEntry? [BEq α] [LawfulBEq α] {l : List (Σ a, β a
     · rw [getValueCast?_cons_of_false h, ih, Option.dmap_congr (getEntry?_cons_of_false h)]
     · rw [getValueCast?_cons_of_true h, Option.dmap_congr (getEntry?_cons_of_true h), Option.dmap_some]
 
-theorem isSome_getValueCast?_eq_isSome_getEntry? [BEq α] [LawfulBEq α] {l : List (Σ a, β a)} {a : α} :
+theorem isSome_getValueCast?_eq_isSome_getEntry? [BEq α] [LawfulBEq α] {l : List ((a : α) × β a)} {a : α} :
     (getValueCast? a l).isSome = (getEntry? a l).isSome := by
   rw [getValueCast?_eq_getEntry?, Option.isSome_dmap]
 
-theorem isEmpty_eq_false_iff_exists_isSome_getValueCast? [BEq α] [LawfulBEq α] {l : List (Σ a, β a)} :
+theorem isEmpty_eq_false_iff_exists_isSome_getValueCast? [BEq α] [LawfulBEq α] {l : List ((a : α) × β a)} :
     l.isEmpty = false ↔ ∃ a, (getValueCast? a l).isSome := by
   simp [isEmpty_eq_false_iff_exists_isSome_getEntry?, isSome_getValueCast?_eq_isSome_getEntry?]
 
-def containsKey [BEq α] (a : α) : List (Σ a, β a) → Bool
+def containsKey [BEq α] (a : α) : List ((a : α) × β a) → Bool
   | [] => false
   | ⟨k, _⟩ :: l => a == k || containsKey a l
 
-@[simp] theorem containsKey_nil [BEq α] {a : α} : containsKey a ([] : List (Σ a, β a)) = false := rfl
-@[simp] theorem containsKey_cons [BEq α] {l : List (Σ a, β a)} {k a : α} {v : β k} :
+@[simp] theorem containsKey_nil [BEq α] {a : α} : containsKey a ([] : List ((a : α) × β a)) = false := rfl
+@[simp] theorem containsKey_cons [BEq α] {l : List ((a : α) × β a)} {k a : α} {v : β k} :
     containsKey a (⟨k, v⟩ :: l) = (a == k || containsKey a l) := rfl
 
-theorem containsKey_cons_eq_false [BEq α] {l : List (Σ a, β a)} {k a : α} {v : β k} :
+theorem containsKey_cons_eq_false [BEq α] {l : List ((a : α) × β a)} {k a : α} {v : β k} :
     (containsKey a (⟨k, v⟩ :: l) = false) ↔ ((a == k) = false) ∧ (containsKey a l = false) := by
   simp [containsKey_cons, not_or]
 
-theorem containsKey_cons_eq_true [BEq α] {l : List (Σ a, β a)} {k a : α} {v : β k} :
+theorem containsKey_cons_eq_true [BEq α] {l : List ((a : α) × β a)} {k a : α} {v : β k} :
     (containsKey a (⟨k, v⟩ :: l)) ↔ (a == k) ∨ (containsKey a l) := by
   simp [containsKey_cons]
 
-theorem containsKey_cons_of_beq [BEq α] {l : List (Σ a, β a)} {k a : α} {v : β k} (h : a == k) :
+theorem containsKey_cons_of_beq [BEq α] {l : List ((a : α) × β a)} {k a : α} {v : β k} (h : a == k) :
     containsKey a (⟨k, v⟩ :: l) := containsKey_cons_eq_true.2 <| Or.inl h
 
 @[simp]
-theorem containsKey_cons_self [BEq α] [ReflBEq α] {l : List (Σ a, β a)} {k : α} {v : β k} :
+theorem containsKey_cons_self [BEq α] [ReflBEq α] {l : List ((a : α) × β a)} {k : α} {v : β k} :
     containsKey k (⟨k, v⟩ :: l) := containsKey_cons_of_beq BEq.refl
 
-theorem containsKey_cons_of_containsKey [BEq α] {l : List (Σ a, β a)} {k a : α} {v : β k} (h : containsKey a l) :
+theorem containsKey_cons_of_containsKey [BEq α] {l : List ((a : α) × β a)} {k a : α} {v : β k} (h : containsKey a l) :
     containsKey a (⟨k, v⟩ :: l) := containsKey_cons_eq_true.2 <| Or.inr h
 
-theorem containsKey_of_containsKey_cons [BEq α] {l : List (Σ a, β a)} {k a : α} {v : β k} (h₁ : containsKey a (⟨k, v⟩ :: l))
+theorem containsKey_of_containsKey_cons [BEq α] {l : List ((a : α) × β a)} {k a : α} {v : β k} (h₁ : containsKey a (⟨k, v⟩ :: l))
     (h₂ : (a == k) = false) : containsKey a l := by
   rcases (containsKey_cons_eq_true.1 h₁) with (h|h)
   · exact False.elim (Bool.eq_false_iff.1 h₂ h)
   · exact h
 
-theorem containsKey_eq_isSome_getEntry? [BEq α] {l : List (Σ a, β a)} {a : α} :
+theorem containsKey_eq_isSome_getEntry? [BEq α] {l : List ((a : α) × β a)} {a : α} :
     containsKey a l = (getEntry? a l).isSome := by
   induction l using assoc_induction
   · simp
@@ -235,16 +235,16 @@ theorem containsKey_eq_isSome_getEntry? [BEq α] {l : List (Σ a, β a)} {a : α
     · simp [getEntry?_cons_of_false h, h, ih]
     · simp [getEntry?_cons_of_true h, h]
 
-theorem isEmpty_eq_false_of_containsKey [BEq α] {l : List (Σ a, β a)} {a : α} (h : containsKey a l = true) :
+theorem isEmpty_eq_false_of_containsKey [BEq α] {l : List ((a : α) × β a)} {a : α} (h : containsKey a l = true) :
     l.isEmpty = false := by
   cases l <;> simp_all
 
-theorem isEmpty_eq_false_iff_exists_containsKey [BEq α] [ReflBEq α] {l : List (Σ a, β a)} :
+theorem isEmpty_eq_false_iff_exists_containsKey [BEq α] [ReflBEq α] {l : List ((a : α) × β a)} :
     l.isEmpty = false ↔ ∃ a, containsKey a l := by
   simp [isEmpty_eq_false_iff_exists_isSome_getEntry?, containsKey_eq_isSome_getEntry?]
 
 @[simp]
-theorem getEntry?_eq_none [BEq α] {l : List (Σ a, β a)} {a : α} :
+theorem getEntry?_eq_none [BEq α] {l : List ((a : α) × β a)} {a : α} :
     getEntry? a l = none ↔ containsKey a l = false := by
   rw [← Option.not_isSome_iff_eq_none, Bool.not_eq_true, ← containsKey_eq_isSome_getEntry?]
 
@@ -257,43 +257,43 @@ theorem containsKey_eq_isSome_getValue? {β : Type v} [BEq α] {l : List ((_ : �
     containsKey a l = (getValue? a l).isSome := by
   simp [containsKey_eq_isSome_getEntry?, getValue?_eq_getEntry?]
 
-theorem containsKey_eq_isSome_getValueCast? [BEq α] [LawfulBEq α] {l : List (Σ a, β a)} {a : α} :
+theorem containsKey_eq_isSome_getValueCast? [BEq α] [LawfulBEq α] {l : List ((a : α) × β a)} {a : α} :
     containsKey a l = (getValueCast? a l).isSome := by
   simp [containsKey_eq_isSome_getEntry?, getValueCast?_eq_getEntry?]
 
-theorem getValueCast?_eq_none [BEq α] [LawfulBEq α] {l : List (Σ a, β a)} {a : α}
+theorem getValueCast?_eq_none [BEq α] [LawfulBEq α] {l : List ((a : α) × β a)} {a : α}
     (h : containsKey a l = false) : getValueCast? a l = none := by
   rwa [← Option.not_isSome_iff_eq_none, ← containsKey_eq_isSome_getValueCast?, Bool.not_eq_true]
 
-theorem containsKey_congr [BEq α] [PartialEquivBEq α] {l : List (Σ a, β a)} {a b : α} (h : a == b) :
+theorem containsKey_congr [BEq α] [PartialEquivBEq α] {l : List ((a : α) × β a)} {a b : α} (h : a == b) :
     containsKey a l = containsKey b l := by
   simp [containsKey_eq_isSome_getEntry?, getEntry?_congr h]
 
-theorem containsKey_of_beq [BEq α] [PartialEquivBEq α] {l : List (Σ a, β a)} {a b : α} (hla : containsKey a l) (hab : a == b) :
+theorem containsKey_of_beq [BEq α] [PartialEquivBEq α] {l : List ((a : α) × β a)} {a b : α} (hla : containsKey a l) (hab : a == b) :
     containsKey b l := by
   rwa [← containsKey_congr hab]
 
-def getEntry [BEq α] (a : α) (l : List (Σ a, β a)) (h : containsKey a l) : Σ a, β a :=
+def getEntry [BEq α] (a : α) (l : List ((a : α) × β a)) (h : containsKey a l) : (a : α) × β a :=
   (getEntry? a l).get <| containsKey_eq_isSome_getEntry?.symm.trans h
 
-theorem getEntry?_eq_some_getEntry [BEq α] {l : List (Σ a, β a)} {a : α} (h : containsKey a l) :
+theorem getEntry?_eq_some_getEntry [BEq α] {l : List ((a : α) × β a)} {a : α} (h : containsKey a l) :
     getEntry? a l = some (getEntry a l h) := by
   simp [getEntry]
 
-theorem getEntry_eq_of_getEntry?_eq_some [BEq α] {l : List (Σ a, β a)} {k a : α} {v : β k}
+theorem getEntry_eq_of_getEntry?_eq_some [BEq α] {l : List ((a : α) × β a)} {k a : α} {v : β k}
     (h : getEntry? a l = some ⟨k, v⟩) {h'} : getEntry a l h' = ⟨k, v⟩ := by
   simp [getEntry, h]
 
-theorem getEntry_cons_of_beq [BEq α] {l : List (Σ a, β a)} {k a : α} {v : β k} (h : a == k) :
+theorem getEntry_cons_of_beq [BEq α] {l : List ((a : α) × β a)} {k a : α} {v : β k} (h : a == k) :
     getEntry a (⟨k, v⟩ :: l) (containsKey_cons_of_beq (v := v) h) = ⟨k, v⟩ := by
   simp [getEntry, getEntry?_cons_of_true h]
 
 @[simp]
-theorem getEntry_cons_self [BEq α] [ReflBEq α] {l : List (Σ a, β a)} {k : α} {v : β k} :
+theorem getEntry_cons_self [BEq α] [ReflBEq α] {l : List ((a : α) × β a)} {k : α} {v : β k} :
     getEntry k (⟨k, v⟩ :: l) containsKey_cons_self = ⟨k, v⟩ :=
   getEntry_cons_of_beq BEq.refl
 
-theorem getEntry_cons_of_false [BEq α] {l : List (Σ a, β a)} {k a : α} {v : β k} {h₁ : containsKey a (⟨k, v⟩ :: l)}
+theorem getEntry_cons_of_false [BEq α] {l : List ((a : α) × β a)} {k a : α} {v : β k} {h₁ : containsKey a (⟨k, v⟩ :: l)}
     (h₂ : (a == k) = false) :
     getEntry a (⟨k, v⟩ :: l) h₁ = getEntry a l (containsKey_of_containsKey_cons (v := v) h₁ h₂) := by
   simp [getEntry, getEntry?_cons_of_false h₂]
@@ -335,17 +335,17 @@ theorem getValue_congr [BEq α] [PartialEquivBEq α] {l : List ((_ : α) × β)}
 
 end
 
-def getValueCast [BEq α] [LawfulBEq α] (a : α) (l : List (Σ a, β a)) (h : containsKey a l) : β a :=
+def getValueCast [BEq α] [LawfulBEq α] (a : α) (l : List ((a : α) × β a)) (h : containsKey a l) : β a :=
   (getValueCast? a l).get <| containsKey_eq_isSome_getValueCast?.symm.trans h
 
-theorem getValueCast?_eq_some_getValueCast [BEq α] [LawfulBEq α] {l : List (Σ a, β a)} {a : α} (h : containsKey a l) :
+theorem getValueCast?_eq_some_getValueCast [BEq α] [LawfulBEq α] {l : List ((a : α) × β a)} {a : α} (h : containsKey a l) :
     getValueCast? a l = some (getValueCast a l h) := by
   simp [getValueCast]
 
 theorem Option.get_congr {o o' : Option α} {ho : o.isSome} (h : o = o') : o.get ho = o'.get (h ▸ ho) := by
   cases h; rfl
 
-theorem getValueCast_cons [BEq α] [LawfulBEq α] {l : List (Σ a, β a)} {k a : α} {v : β k}
+theorem getValueCast_cons [BEq α] [LawfulBEq α] {l : List ((a : α) × β a)} {k a : α} {v : β k}
     (h : containsKey a (⟨k, v⟩ :: l)) :
     getValueCast a (⟨k, v⟩ :: l) h =
       if h' : a == k then
@@ -361,51 +361,51 @@ theorem getValue_eq_getValueCast {β : Type v} [BEq α] [LawfulBEq α] {l : List
   · simp at h
   · simp_all [getValue_cons, getValueCast_cons]
 
-def getValueCastD [BEq α] [LawfulBEq α] (a : α) (l : List (Σ a, β a)) (fallback : β a) : β a :=
+def getValueCastD [BEq α] [LawfulBEq α] (a : α) (l : List ((a : α) × β a)) (fallback : β a) : β a :=
   (getValueCast? a l).getD fallback
 
 @[simp]
-theorem getValueCastD_nil [BEq α] [LawfulBEq α] {a : α} {fallback : β a} : getValueCastD a ([] : List (Σ a, β a)) fallback = fallback := rfl
+theorem getValueCastD_nil [BEq α] [LawfulBEq α] {a : α} {fallback : β a} : getValueCastD a ([] : List ((a : α) × β a)) fallback = fallback := rfl
 
-theorem getValueCastD_eq_getValueCast? [BEq α] [LawfulBEq α] {l : List (Σ a, β a)} {a : α} {fallback : β a} :
+theorem getValueCastD_eq_getValueCast? [BEq α] [LawfulBEq α] {l : List ((a : α) × β a)} {a : α} {fallback : β a} :
     getValueCastD a l fallback = (getValueCast? a l).getD fallback := rfl
 
-theorem getValueCastD_eq_fallback [BEq α] [LawfulBEq α] {l : List (Σ a, β a)} {a : α} {fallback : β a}
+theorem getValueCastD_eq_fallback [BEq α] [LawfulBEq α] {l : List ((a : α) × β a)} {a : α} {fallback : β a}
     (h : containsKey a l = false) : getValueCastD a l fallback = fallback := by
   rw [containsKey_eq_isSome_getValueCast?, Bool.eq_false_iff, ne_eq, Option.not_isSome_iff_eq_none] at h
   rw [getValueCastD_eq_getValueCast?, h, Option.getD_none]
 
-theorem getValueCast_eq_getValueCastD [BEq α] [LawfulBEq α] {l : List (Σ a, β a)} {a : α} {fallback : β a}
+theorem getValueCast_eq_getValueCastD [BEq α] [LawfulBEq α] {l : List ((a : α) × β a)} {a : α} {fallback : β a}
     (h : containsKey a l = true) : getValueCast a l h = getValueCastD a l fallback := by
   rw [getValueCastD_eq_getValueCast?, getValueCast, Option.get_eq_getD]
 
-theorem getValueCast?_eq_some_getValueCastD [BEq α] [LawfulBEq α] {l : List (Σ a, β a)} {a : α} {fallback : β a}
+theorem getValueCast?_eq_some_getValueCastD [BEq α] [LawfulBEq α] {l : List ((a : α) × β a)} {a : α} {fallback : β a}
     (h : containsKey a l = true) : getValueCast? a l = some (getValueCastD a l fallback) := by
   rw [getValueCast?_eq_some_getValueCast h, getValueCast_eq_getValueCastD]
 
-def getValueCast! [BEq α] [LawfulBEq α] (a : α) [Inhabited (β a)] (l : List (Σ a, β a)) : β a :=
+def getValueCast! [BEq α] [LawfulBEq α] (a : α) [Inhabited (β a)] (l : List ((a : α) × β a)) : β a :=
   (getValueCast? a l).get!
 
 @[simp]
-theorem getValueCast!_nil [BEq α] [LawfulBEq α] {a : α} [Inhabited (β a)] : getValueCast! a ([] : List (Σ a, β a)) = default := rfl
+theorem getValueCast!_nil [BEq α] [LawfulBEq α] {a : α} [Inhabited (β a)] : getValueCast! a ([] : List ((a : α) × β a)) = default := rfl
 
-theorem getValueCast!_eq_getValueCast? [BEq α] [LawfulBEq α] {l : List (Σ a, β a)} {a : α} [Inhabited (β a)] :
+theorem getValueCast!_eq_getValueCast? [BEq α] [LawfulBEq α] {l : List ((a : α) × β a)} {a : α} [Inhabited (β a)] :
     getValueCast! a l = (getValueCast? a l).get! := rfl
 
-theorem getValueCast!_eq_default [BEq α] [LawfulBEq α] {l : List (Σ a, β a)} {a : α} [Inhabited (β a)]
+theorem getValueCast!_eq_default [BEq α] [LawfulBEq α] {l : List ((a : α) × β a)} {a : α} [Inhabited (β a)]
     (h : containsKey a l = false) : getValueCast! a l = default := by
   rw [containsKey_eq_isSome_getValueCast?, Bool.eq_false_iff, ne_eq, Option.not_isSome_iff_eq_none] at h
   rw [getValueCast!_eq_getValueCast?, h, Option.get!_none]
 
-theorem getValueCast_eq_getValueCast! [BEq α] [LawfulBEq α] {l : List (Σ a, β a)} {a : α} [Inhabited (β a)]
+theorem getValueCast_eq_getValueCast! [BEq α] [LawfulBEq α] {l : List ((a : α) × β a)} {a : α} [Inhabited (β a)]
     (h : containsKey a l = true) : getValueCast a l h = getValueCast! a l := by
   rw [getValueCast!_eq_getValueCast?, getValueCast, Option.get_eq_get!]
 
-theorem getValueCast?_eq_some_getValueCast! [BEq α] [LawfulBEq α] {l : List (Σ a, β a)} {a : α} [Inhabited (β a)]
+theorem getValueCast?_eq_some_getValueCast! [BEq α] [LawfulBEq α] {l : List ((a : α) × β a)} {a : α} [Inhabited (β a)]
     (h : containsKey a l = true) : getValueCast? a l = some (getValueCast! a l) := by
   rw [getValueCast?_eq_some_getValueCast h, getValueCast_eq_getValueCast!]
 
-theorem getValueCast!_eq_getValueCastD_default [BEq α] [LawfulBEq α] {l : List (Σ a, β a)} {a : α} [Inhabited (β a)] :
+theorem getValueCast!_eq_getValueCastD_default [BEq α] [LawfulBEq α] {l : List ((a : α) × β a)} {a : α} [Inhabited (β a)] :
     getValueCast! a l = getValueCastD a l default := rfl
 
 section
@@ -477,23 +477,23 @@ theorem getValue!_eq_getValueD_default [BEq α] [Inhabited β] {l : List ((_ : �
 
 end
 
-def replaceEntry [BEq α] (k : α) (v : β k) : List (Σ a, β a) → List (Σ a, β a)
+def replaceEntry [BEq α] (k : α) (v : β k) : List ((a : α) × β a) → List ((a : α) × β a)
   | [] => []
   | ⟨k', v'⟩ :: l => bif k == k' then ⟨k, v⟩ :: l else ⟨k', v'⟩ :: replaceEntry k v l
 
 @[simp] theorem replaceEntry_nil [BEq α] {k : α} {v : β k} : replaceEntry k v [] = [] := rfl
-theorem replaceEntry_cons [BEq α] {l : List (Σ a, β a)} {k k' : α} {v : β k} {v' : β k'} :
+theorem replaceEntry_cons [BEq α] {l : List ((a : α) × β a)} {k k' : α} {v : β k} {v' : β k'} :
     replaceEntry k v (⟨k', v'⟩ :: l) = bif k == k' then ⟨k, v⟩ :: l else ⟨k', v'⟩ :: replaceEntry k v l := rfl
 
-theorem replaceEntry_cons_of_true [BEq α] {l : List (Σ a, β a)} {k k' : α} {v : β k} {v' : β k'} (h : k == k') :
+theorem replaceEntry_cons_of_true [BEq α] {l : List ((a : α) × β a)} {k k' : α} {v : β k} {v' : β k'} (h : k == k') :
     replaceEntry k v (⟨k', v'⟩ :: l) = ⟨k, v⟩ :: l := by
   simp [replaceEntry, h]
 
-theorem replaceEntry_cons_of_false [BEq α] {l : List (Σ a, β a)} {k k' : α} {v : β k} {v' : β k'} (h : (k == k') = false) :
+theorem replaceEntry_cons_of_false [BEq α] {l : List ((a : α) × β a)} {k k' : α} {v : β k} {v' : β k'} (h : (k == k') = false) :
     replaceEntry k v (⟨k', v'⟩ :: l) = ⟨k', v'⟩ :: replaceEntry k v l := by
   simp [replaceEntry, h]
 
-theorem replaceEntry_of_containsKey_eq_false [BEq α] {l : List (Σ a, β a)} {k : α} {v : β k} (h : containsKey k l = false) :
+theorem replaceEntry_of_containsKey_eq_false [BEq α] {l : List ((a : α) × β a)} {k : α} {v : β k} (h : containsKey k l = false) :
     replaceEntry k v l = l := by
   induction l
   · simp
@@ -502,17 +502,17 @@ theorem replaceEntry_of_containsKey_eq_false [BEq α] {l : List (Σ a, β a)} {k
     rw [replaceEntry_cons_of_false h.1, ih h.2]
 
 @[simp]
-theorem isEmpty_replaceEntry [BEq α] {l : List (Σ a, β a)} {k : α} {v : β k} : (replaceEntry k v l).isEmpty = l.isEmpty := by
+theorem isEmpty_replaceEntry [BEq α] {l : List ((a : α) × β a)} {k : α} {v : β k} : (replaceEntry k v l).isEmpty = l.isEmpty := by
   induction l using assoc_induction
   · simp
   · simp [replaceEntry_cons, cond_eq_if]
     split <;> simp
 
-theorem getEntry?_replaceEntry_of_containsKey_eq_false [BEq α] {l : List (Σ a, β a)} {a k : α} {v : β k}
+theorem getEntry?_replaceEntry_of_containsKey_eq_false [BEq α] {l : List ((a : α) × β a)} {a k : α} {v : β k}
     (hl : containsKey k l = false) : getEntry? a (replaceEntry k v l) = getEntry? a l := by
   rw [replaceEntry_of_containsKey_eq_false hl]
 
-theorem getEntry?_replaceEntry_of_false [BEq α] [PartialEquivBEq α] {l : List (Σ a, β a)} {a k : α} {v : β k}
+theorem getEntry?_replaceEntry_of_false [BEq α] [PartialEquivBEq α] {l : List ((a : α) × β a)} {a k : α} {v : β k}
     (h : (a == k) = false) : getEntry? a (replaceEntry k v l) = getEntry? a l := by
   induction l using assoc_induction
   · simp
@@ -523,7 +523,7 @@ theorem getEntry?_replaceEntry_of_false [BEq α] [PartialEquivBEq α] {l : List 
       have hk : (a == k') = false := BEq.neq_of_neq_of_beq h h'
       simp [getEntry?_cons_of_false h, getEntry?_cons_of_false hk]
 
-theorem getEntry?_replaceEntry_of_true [BEq α] [PartialEquivBEq α] {l : List (Σ a, β a)} {a k : α} {v : β k} (hl : containsKey k l = true)
+theorem getEntry?_replaceEntry_of_true [BEq α] [PartialEquivBEq α] {l : List ((a : α) × β a)} {a k : α} {v : β k} (hl : containsKey k l = true)
     (h : a == k) : getEntry? a (replaceEntry k v l) = some ⟨k, v⟩ := by
   induction l using assoc_induction
   · simp at hl
@@ -535,7 +535,7 @@ theorem getEntry?_replaceEntry_of_true [BEq α] [PartialEquivBEq α] {l : List (
       exact ih (containsKey_of_containsKey_cons hl hk'a)
     · rw [replaceEntry_cons_of_true hk'a, getEntry?_cons_of_true h]
 
-theorem getEntry?_replaceEntry [BEq α] [PartialEquivBEq α] {l : List (Σ a, β a)} {a k : α} {v : β k} :
+theorem getEntry?_replaceEntry [BEq α] [PartialEquivBEq α] {l : List ((a : α) × β a)} {a k : α} {v : β k} :
     getEntry? a (replaceEntry k v l) = bif containsKey k l && a == k then some ⟨k, v⟩ else
       getEntry? a l := by
   cases hl : containsKey k l
@@ -545,7 +545,7 @@ theorem getEntry?_replaceEntry [BEq α] [PartialEquivBEq α] {l : List (Σ a, β
     · simp [getEntry?_replaceEntry_of_true hl h]
 
 @[simp]
-theorem length_replaceEntry [BEq α] {l : List (Σ a, β a)} {k : α} {v : β k} :
+theorem length_replaceEntry [BEq α] {l : List ((a : α) × β a)} {k : α} {v : β k} :
     (replaceEntry k v l).length = l.length := by
   induction l using assoc_induction <;> simp_all [replaceEntry_cons, apply_bif List.length]
 
@@ -567,7 +567,7 @@ theorem getValue?_replaceEntry_of_true [BEq α] [PartialEquivBEq α] {l : List (
 
 end
 
-theorem getValueCast?_replaceEntry [BEq α] [LawfulBEq α] {l : List (Σ a, β a)} {a k : α} {v : β k} :
+theorem getValueCast?_replaceEntry [BEq α] [LawfulBEq α] {l : List ((a : α) × β a)} {a k : α} {v : β k} :
     getValueCast? a (replaceEntry k v l) =
       if h : containsKey k l ∧ a == k then some (cast (congrArg β (eq_of_beq h.2).symm) v) else getValueCast? a l := by
   rw [getValueCast?_eq_getEntry?]
@@ -583,7 +583,7 @@ theorem getValueCast?_replaceEntry [BEq α] [LawfulBEq α] {l : List (Σ a, β a
         getValueCast?_eq_getEntry?]
 
 @[simp]
-theorem containsKey_replaceEntry [BEq α] [PartialEquivBEq α] {l : List (Σ a, β a)} {a k : α} {v : β k} :
+theorem containsKey_replaceEntry [BEq α] [PartialEquivBEq α] {l : List ((a : α) × β a)} {a k : α} {v : β k} :
     containsKey a (replaceEntry k v l) = containsKey a l := by
   cases h : containsKey k l && a == k
   · rw [containsKey_eq_isSome_getEntry?, getEntry?_replaceEntry, h, cond_false, containsKey_eq_isSome_getEntry?]
@@ -591,28 +591,28 @@ theorem containsKey_replaceEntry [BEq α] [PartialEquivBEq α] {l : List (Σ a, 
     rw [Bool.and_eq_true] at h
     exact containsKey_of_beq h.1 (BEq.symm h.2)
 
-def removeKey [BEq α] (k : α) : List (Σ a, β a) → List (Σ a, β a)
+def removeKey [BEq α] (k : α) : List ((a : α) × β a) → List ((a : α) × β a)
   | [] => []
   | ⟨k', v'⟩ :: l => bif k == k' then l else ⟨k', v'⟩ :: removeKey k l
 
-@[simp] theorem removeKey_nil [BEq α] {k : α} : removeKey k ([] : List (Σ a, β a)) = [] := rfl
-theorem removeKey_cons [BEq α] {l : List (Σ a, β a)} {k k' : α} {v' : β k'} :
+@[simp] theorem removeKey_nil [BEq α] {k : α} : removeKey k ([] : List ((a : α) × β a)) = [] := rfl
+theorem removeKey_cons [BEq α] {l : List ((a : α) × β a)} {k k' : α} {v' : β k'} :
     removeKey k (⟨k', v'⟩ :: l) = bif k == k' then l else ⟨k', v'⟩ :: removeKey k l := rfl
 
-theorem removeKey_cons_of_beq [BEq α] {l : List (Σ a, β a)} {k k' : α} {v' : β k'} (h : k == k') :
+theorem removeKey_cons_of_beq [BEq α] {l : List ((a : α) × β a)} {k k' : α} {v' : β k'} (h : k == k') :
     removeKey k (⟨k', v'⟩ :: l) = l :=
   by simp [removeKey_cons, h]
 
 @[simp]
-theorem removeKey_cons_self [BEq α] [ReflBEq α] {l : List (Σ a, β a)} {k : α} {v : β k} :
+theorem removeKey_cons_self [BEq α] [ReflBEq α] {l : List ((a : α) × β a)} {k : α} {v : β k} :
     removeKey k (⟨k, v⟩ :: l) = l :=
   removeKey_cons_of_beq BEq.refl
 
-theorem removeKey_cons_of_false [BEq α] {l : List (Σ a, β a)} {k k' : α} {v' : β k'} (h : (k == k') = false) :
+theorem removeKey_cons_of_false [BEq α] {l : List ((a : α) × β a)} {k k' : α} {v' : β k'} (h : (k == k') = false) :
     removeKey k (⟨k', v'⟩ :: l) = ⟨k', v'⟩ :: removeKey k l := by
   simp [removeKey_cons, h]
 
-theorem removeKey_of_containsKey_eq_false [BEq α] {l : List (Σ a, β a)} {k : α} (h : containsKey k l = false) :
+theorem removeKey_of_containsKey_eq_false [BEq α] {l : List ((a : α) × β a)} {k : α} (h : containsKey k l = false) :
     removeKey k l = l := by
   induction l using assoc_induction
   · simp
@@ -620,7 +620,7 @@ theorem removeKey_of_containsKey_eq_false [BEq α] {l : List (Σ a, β a)} {k : 
     simp only [containsKey_cons, Bool.or_eq_false_iff] at h
     rw [removeKey_cons_of_false h.1, ih h.2]
 
-theorem sublist_removeKey [BEq α] {l : List (Σ a, β a)} {k : α} : Sublist (removeKey k l) l := by
+theorem sublist_removeKey [BEq α] {l : List ((a : α) × β a)} {k : α} : Sublist (removeKey k l) l := by
   induction l using assoc_induction
   · simp
   · next k' v' t ih =>
@@ -629,7 +629,7 @@ theorem sublist_removeKey [BEq α] {l : List (Σ a, β a)} {k : α} : Sublist (r
     · simpa
     · simpa using Sublist.cons_right Sublist.refl
 
-theorem length_removeKey [BEq α] {l : List (Σ a, β a)} {k : α} :
+theorem length_removeKey [BEq α] {l : List ((a : α) × β a)} {k : α} :
     (removeKey k l).length = bif containsKey k l then l.length - 1 else l.length := by
   induction l using assoc_induction
   · simp
@@ -646,75 +646,75 @@ theorem length_removeKey [BEq α] {l : List (Σ a, β a)} {k : α} :
         · simp
     · simp
 
-theorem length_removeKey_le [BEq α] {l : List (Σ a, β a)} {k : α} :
+theorem length_removeKey_le [BEq α] {l : List ((a : α) × β a)} {k : α} :
     (removeKey k l).length ≤ l.length :=
   sublist_removeKey.length_le
 
-theorem isEmpty_removeKey [BEq α] {l : List (Σ a, β a)} {k : α} :
+theorem isEmpty_removeKey [BEq α] {l : List ((a : α) × β a)} {k : α} :
     (removeKey k l).isEmpty = (l.isEmpty || (l.length == 1 && containsKey k l)) := by
   rw [Bool.eq_iff_iff]
   simp only [Bool.or_eq_true, Bool.and_eq_true, beq_iff_eq]
   rw [List.isEmpty_iff_length_eq_zero, length_removeKey, List.isEmpty_iff_length_eq_zero]
   cases containsKey k l <;> cases l <;> simp
 
-@[simp] theorem keys_nil : keys ([] : List (Σ a, β a)) = [] := rfl
-@[simp] theorem keys_cons {l : List (Σ a, β a)} {k : α} {v : β k} : keys (⟨k, v⟩ :: l) = k :: keys l := rfl
+@[simp] theorem keys_nil : keys ([] : List ((a : α) × β a)) = [] := rfl
+@[simp] theorem keys_cons {l : List ((a : α) × β a)} {k : α} {v : β k} : keys (⟨k, v⟩ :: l) = k :: keys l := rfl
 
-theorem keys_eq_map (l : List (Σ a, β a)) : keys l = l.map (·.1) := by
+theorem keys_eq_map (l : List ((a : α) × β a)) : keys l = l.map (·.1) := by
   induction l using assoc_induction <;> simp_all
 
-theorem containsKey_eq_keys_contains [BEq α] [PartialEquivBEq α] {l : List (Σ a, β a)} {a : α} :
+theorem containsKey_eq_keys_contains [BEq α] [PartialEquivBEq α] {l : List ((a : α) × β a)} {a : α} :
     containsKey a l = (keys l).contains a := by
   induction l using assoc_induction
   · rfl
   · next k _ l ih => simp [ih, BEq.comm]
 
-theorem containsKey_eq_true_iff_exists_mem [BEq α] {l : List (Σ a, β a)} {a : α} :
+theorem containsKey_eq_true_iff_exists_mem [BEq α] {l : List ((a : α) × β a)} {a : α} :
     containsKey a l = true ↔ ∃ p ∈ l, a == p.1 := by
   induction l using assoc_induction <;> simp_all
 
-theorem containsKey_of_mem [BEq α] [ReflBEq α] {l : List (Σ a, β a)} {p : Σ a, β a} (hp : p ∈ l) :
+theorem containsKey_of_mem [BEq α] [ReflBEq α] {l : List ((a : α) × β a)} {p : (a : α) × β a} (hp : p ∈ l) :
     containsKey p.1 l :=
   containsKey_eq_true_iff_exists_mem.2 ⟨p, ⟨hp, BEq.refl⟩⟩
 
 @[simp]
-theorem DistinctKeys.nil [BEq α] : DistinctKeys ([] : List (Σ a, β a)) :=
+theorem DistinctKeys.nil [BEq α] : DistinctKeys ([] : List ((a : α) × β a)) :=
   ⟨by simp⟩
 
 open List
 
-theorem DistinctKeys.perm_keys [BEq α] [PartialEquivBEq α] {l l' : List (Σ a, β a)}
+theorem DistinctKeys.perm_keys [BEq α] [PartialEquivBEq α] {l l' : List ((a : α) × β a)}
     (h : Perm (keys l') (keys l)) : DistinctKeys l → DistinctKeys l'
   | ⟨h'⟩ => ⟨h'.perm BEq.symm_false h.symm⟩
 
-theorem DistinctKeys.perm [BEq α] [PartialEquivBEq α] {l l' : List (Σ a, β a)} (h : Perm l' l) :
+theorem DistinctKeys.perm [BEq α] [PartialEquivBEq α] {l l' : List ((a : α) × β a)} (h : Perm l' l) :
     DistinctKeys l → DistinctKeys l' :=
   DistinctKeys.perm_keys (by simpa only [keys_eq_map] using h.map _)
 
-theorem DistinctKeys.congr [BEq α] [PartialEquivBEq α] {l l' : List (Σ a, β a)} (h : Perm l l') :
+theorem DistinctKeys.congr [BEq α] [PartialEquivBEq α] {l l' : List ((a : α) × β a)} (h : Perm l l') :
     DistinctKeys l ↔ DistinctKeys l' :=
   ⟨fun h' => h'.perm h.symm, fun h' => h'.perm h⟩
 
-theorem distinctKeys_of_sublist_keys [BEq α] {l : List (Σ a, β a)} {l' : List (Σ a, γ a)}
+theorem distinctKeys_of_sublist_keys [BEq α] {l : List ((a : α) × β a)} {l' : List ((a : α) × γ a)}
     (h : Sublist (keys l') (keys l)) : DistinctKeys l → DistinctKeys l' :=
   fun ⟨h'⟩ => ⟨h'.sublist h⟩
 
-theorem distinctKeys_of_sublist [BEq α] {l l' : List (Σ a, β a)} (h : Sublist l' l) : DistinctKeys l → DistinctKeys l' :=
+theorem distinctKeys_of_sublist [BEq α] {l l' : List ((a : α) × β a)} (h : Sublist l' l) : DistinctKeys l → DistinctKeys l' :=
   distinctKeys_of_sublist_keys (by simpa only [keys_eq_map] using h.map _)
 
-theorem DistinctKeys.of_keys_eq [BEq α] {l : List (Σ a, β a)} {l' : List (Σ a, γ a)} (h : keys l = keys l') : DistinctKeys l → DistinctKeys l' :=
+theorem DistinctKeys.of_keys_eq [BEq α] {l : List ((a : α) × β a)} {l' : List ((a : α) × γ a)} (h : keys l = keys l') : DistinctKeys l → DistinctKeys l' :=
   distinctKeys_of_sublist_keys (h ▸ Sublist.refl)
 
-theorem containsKey_iff_exists [BEq α] [PartialEquivBEq α] {l : List (Σ a, β a)} {a : α} :
+theorem containsKey_iff_exists [BEq α] [PartialEquivBEq α] {l : List ((a : α) × β a)} {a : α} :
     containsKey a l ↔ ∃ a' ∈ keys l, a == a' := by
   rw [containsKey_eq_keys_contains, List.contains_iff_exists_mem_beq]
 
-theorem containsKey_eq_false_iff_forall_mem_keys [BEq α] [PartialEquivBEq α] {l : List (Σ a, β a)} {a : α} :
+theorem containsKey_eq_false_iff_forall_mem_keys [BEq α] [PartialEquivBEq α] {l : List ((a : α) × β a)} {a : α} :
     (containsKey a l) = false ↔ ∀ a' ∈ keys l, (a == a') = false := by
   simp only [Bool.eq_false_iff, ne_eq, containsKey_iff_exists, not_exists, not_and]
 
 @[simp]
-theorem distinctKeys_cons_iff [BEq α] [PartialEquivBEq α] {l : List (Σ a, β a)} {k : α} {v : β k} :
+theorem distinctKeys_cons_iff [BEq α] [PartialEquivBEq α] {l : List ((a : α) × β a)} {k : α} {v : β k} :
     DistinctKeys (⟨k, v⟩ :: l) ↔ DistinctKeys l ∧ (containsKey k l) = false := by
   refine ⟨fun ⟨h⟩ => ?_, fun ⟨⟨h₁⟩, h₂⟩ => ⟨?_⟩⟩
   · rw [keys_cons, pairwise_cons] at h
@@ -722,19 +722,19 @@ theorem distinctKeys_cons_iff [BEq α] [PartialEquivBEq α] {l : List (Σ a, β 
   · rw [keys_cons, pairwise_cons, ← containsKey_eq_false_iff_forall_mem_keys]
     exact ⟨h₂, h₁⟩
 
-theorem DistinctKeys.tail [BEq α] [PartialEquivBEq α] {l : List (Σ a, β a)} {k : α} {v : β k} :
+theorem DistinctKeys.tail [BEq α] [PartialEquivBEq α] {l : List ((a : α) × β a)} {k : α} {v : β k} :
     DistinctKeys (⟨k, v⟩ :: l) → DistinctKeys l :=
   fun h => (distinctKeys_cons_iff.mp h).1
 
-theorem DistinctKeys.containsKey_eq_false [BEq α] [PartialEquivBEq α] {l : List (Σ a, β a)} {k : α} {v : β k} :
+theorem DistinctKeys.containsKey_eq_false [BEq α] [PartialEquivBEq α] {l : List ((a : α) × β a)} {k : α} {v : β k} :
     DistinctKeys (⟨k, v⟩ :: l) → containsKey k l = false :=
   fun h => (distinctKeys_cons_iff.mp h).2
 
-theorem DistinctKeys.cons [BEq α] [PartialEquivBEq α] {l : List (Σ a, β a)} {k : α} {v : β k} (h : containsKey k l = false) :
+theorem DistinctKeys.cons [BEq α] [PartialEquivBEq α] {l : List ((a : α) × β a)} {k : α} {v : β k} (h : containsKey k l = false) :
     DistinctKeys l → DistinctKeys (⟨k, v⟩ :: l) :=
   fun h' => distinctKeys_cons_iff.mpr ⟨h', h⟩
 
-theorem mem_iff_getEntry?_eq_some [BEq α] [EquivBEq α] {l : List (Σ a, β a)} {p : Σ a, β a} (h : DistinctKeys l) :
+theorem mem_iff_getEntry?_eq_some [BEq α] [EquivBEq α] {l : List ((a : α) × β a)} {p : (a : α) × β a} (h : DistinctKeys l) :
     p ∈ l ↔ getEntry? p.1 l = some p := by
   induction l using assoc_induction
   · simp_all
@@ -753,7 +753,7 @@ theorem mem_iff_getEntry?_eq_some [BEq α] [EquivBEq α] {l : List (Σ a, β a)}
       · rw [cond_true, Option.some.injEq]
         exact Or.inl ∘ Eq.symm
 
-theorem DistinctKeys.replaceEntry [BEq α] [PartialEquivBEq α] {l : List (Σ a, β a)} {k : α} {v : β k} (h : DistinctKeys l) :
+theorem DistinctKeys.replaceEntry [BEq α] [PartialEquivBEq α] {l : List ((a : α) × β a)} {k : α} {v : β k} (h : DistinctKeys l) :
     DistinctKeys (replaceEntry k v l) := by
   induction l using assoc_induction
   · simp
@@ -767,22 +767,22 @@ theorem DistinctKeys.replaceEntry [BEq α] [PartialEquivBEq α] {l : List (Σ a,
       refine ⟨h.1, ?_⟩
       simpa [containsKey_congr (BEq.symm hk'k)] using h.2
 
-def insertEntry [BEq α]  (k : α) (v : β k) (l : List (Σ a, β a)) : List (Σ a, β a) :=
+def insertEntry [BEq α]  (k : α) (v : β k) (l : List ((a : α) × β a)) : List ((a : α) × β a) :=
   bif containsKey k l then replaceEntry k v l else ⟨k, v⟩ :: l
 
 @[simp]
-theorem insertEntry_nil [BEq α] {k : α} {v : β k} : insertEntry k v ([] : List (Σ a, β a)) = [⟨k, v⟩] := by
+theorem insertEntry_nil [BEq α] {k : α} {v : β k} : insertEntry k v ([] : List ((a : α) × β a)) = [⟨k, v⟩] := by
   simp [insertEntry]
 
-theorem insertEntry_of_containsKey [BEq α] {l : List (Σ a, β a)} {k : α} {v : β k} (h : containsKey k l) :
+theorem insertEntry_of_containsKey [BEq α] {l : List ((a : α) × β a)} {k : α} {v : β k} (h : containsKey k l) :
     insertEntry k v l = replaceEntry k v l := by
   simp [insertEntry, h]
 
-theorem insertEntry_of_containsKey_eq_false [BEq α] {l : List (Σ a, β a)} {k : α} {v : β k} (h : containsKey k l = false) :
+theorem insertEntry_of_containsKey_eq_false [BEq α] {l : List ((a : α) × β a)} {k : α} {v : β k} (h : containsKey k l = false) :
     insertEntry k v l = ⟨k, v⟩ :: l := by
   simp [insertEntry, h]
 
-theorem DistinctKeys.insertEntry [BEq α] [PartialEquivBEq α] {l : List (Σ a, β a)} {k : α} {v : β k} (h : DistinctKeys l) :
+theorem DistinctKeys.insertEntry [BEq α] [PartialEquivBEq α] {l : List ((a : α) × β a)} {k : α} {v : β k} (h : DistinctKeys l) :
     DistinctKeys (insertEntry k v l) := by
   cases h' : containsKey k l
   · rw [insertEntry_of_containsKey_eq_false h', distinctKeys_cons_iff]
@@ -791,16 +791,16 @@ theorem DistinctKeys.insertEntry [BEq α] [PartialEquivBEq α] {l : List (Σ a, 
     exact h.replaceEntry
 
 @[simp]
-theorem isEmpty_insertEntry [BEq α] {l : List (Σ a, β a)} {k : α} {v : β k} : (insertEntry k v l).isEmpty = false := by
+theorem isEmpty_insertEntry [BEq α] {l : List ((a : α) × β a)} {k : α} {v : β k} : (insertEntry k v l).isEmpty = false := by
   cases h : containsKey k l
   · simp [insertEntry_of_containsKey_eq_false h]
   · rw [insertEntry_of_containsKey h, isEmpty_replaceEntry, isEmpty_eq_false_of_containsKey h]
 
-theorem length_insertEntry [BEq α] {l : List (Σ a, β a)} {k : α} {v : β k} :
+theorem length_insertEntry [BEq α] {l : List ((a : α) × β a)} {k : α} {v : β k} :
     (insertEntry k v l).length = bif containsKey k l then l.length else l.length + 1 := by
   simp [insertEntry, apply_bif List.length]
 
-theorem length_le_length_insertEntry [BEq α] {l : List (Σ a, β a)} {k : α} {v : β k} :
+theorem length_le_length_insertEntry [BEq α] {l : List ((a : α) × β a)} {k : α} {v : β k} :
     l.length ≤ (insertEntry k v l).length := by
   rw [length_insertEntry]
   cases containsKey k l
@@ -839,36 +839,36 @@ theorem getValue?_insertEntry_self [BEq α] [EquivBEq α] {l : List ((_ : α) ×
 
 end
 
-theorem getEntry?_insertEntry [BEq α] [PartialEquivBEq α] {l : List (Σ a, β a)} {k a : α} {v : β k} :
+theorem getEntry?_insertEntry [BEq α] [PartialEquivBEq α] {l : List ((a : α) × β a)} {k a : α} {v : β k} :
     getEntry? a (insertEntry k v l) = bif a == k then some ⟨k, v⟩ else getEntry? a l := by
   cases hl : containsKey k l
   · rw [insertEntry_of_containsKey_eq_false hl, getEntry?_cons]
   · rw [insertEntry_of_containsKey hl, getEntry?_replaceEntry, hl, Bool.true_and, BEq.comm]
 
-theorem getValueCast?_insertEntry [BEq α] [LawfulBEq α] {l : List (Σ a, β a)} {k a : α} {v : β k} :
+theorem getValueCast?_insertEntry [BEq α] [LawfulBEq α] {l : List ((a : α) × β a)} {k a : α} {v : β k} :
     getValueCast? a (insertEntry k v l) = if h : a == k then some (cast (congrArg β (eq_of_beq h).symm) v) else getValueCast? a l := by
   cases hl : containsKey k l
   · rw [insertEntry_of_containsKey_eq_false hl, getValueCast?_cons]
   · rw [insertEntry_of_containsKey hl, getValueCast?_replaceEntry, hl]
     split <;> simp_all
 
-theorem getValueCast?_insertEntry_self [BEq α] [LawfulBEq α] {l : List (Σ a, β a)} {k : α} {v : β k} :
+theorem getValueCast?_insertEntry_self [BEq α] [LawfulBEq α] {l : List ((a : α) × β a)} {k : α} {v : β k} :
     getValueCast? k (insertEntry k v l) = some v := by
   rw [getValueCast?_insertEntry, dif_pos BEq.refl, cast_eq]
 
-theorem getValueCast!_insertEntry [BEq α] [LawfulBEq α] {l : List (Σ a, β a)} {k a : α} [Inhabited (β a)] {v : β k} :
+theorem getValueCast!_insertEntry [BEq α] [LawfulBEq α] {l : List ((a : α) × β a)} {k a : α} [Inhabited (β a)] {v : β k} :
     getValueCast! a (insertEntry k v l) = if h : a == k then cast (congrArg β (eq_of_beq h).symm) v else getValueCast! a l := by
   simp [getValueCast!_eq_getValueCast?, getValueCast?_insertEntry, apply_dite Option.get!]
 
-theorem getValueCast!_insertEntry_self [BEq α] [LawfulBEq α] {l : List (Σ a, β a)} {k : α} [Inhabited (β k)] {v : β k} :
+theorem getValueCast!_insertEntry_self [BEq α] [LawfulBEq α] {l : List ((a : α) × β a)} {k : α} [Inhabited (β k)] {v : β k} :
     getValueCast! k (insertEntry k v l) = v := by
   rw [getValueCast!_insertEntry, dif_pos BEq.refl, cast_eq]
 
-theorem getValueCastD_insertEntry [BEq α] [LawfulBEq α] {l : List (Σ a, β a)} {k a : α} {fallback : β a} {v : β k} :
+theorem getValueCastD_insertEntry [BEq α] [LawfulBEq α] {l : List ((a : α) × β a)} {k a : α} {fallback : β a} {v : β k} :
     getValueCastD a (insertEntry k v l) fallback = if h : a == k then cast (congrArg β (eq_of_beq h).symm) v else getValueCastD a l fallback := by
   simp [getValueCastD_eq_getValueCast?, getValueCast?_insertEntry, apply_dite (fun x => Option.getD x fallback)]
 
-theorem getValueCastD_insertEntry_self [BEq α] [LawfulBEq α] {l : List (Σ a, β a)} {k : α} {fallback : β k} {v : β k} :
+theorem getValueCastD_insertEntry_self [BEq α] [LawfulBEq α] {l : List ((a : α) × β a)} {k : α} {fallback : β k} {v : β k} :
     getValueCastD k (insertEntry k v l) fallback = v := by
   rw [getValueCastD_insertEntry, dif_pos BEq.refl, cast_eq]
 
@@ -889,25 +889,25 @@ theorem getValueD_insertEntry_self {β : Type v} [BEq α] [EquivBEq α] {l : Lis
   rw [getValueD_insertEntry, BEq.refl, cond_true]
 
 @[simp]
-theorem containsKey_insertEntry [BEq α] [PartialEquivBEq α] {l : List (Σ a, β a)} {k a : α} {v : β k} :
+theorem containsKey_insertEntry [BEq α] [PartialEquivBEq α] {l : List ((a : α) × β a)} {k a : α} {v : β k} :
     containsKey a (insertEntry k v l) = ((a == k) || containsKey a l) := by
   rw [containsKey_eq_isSome_getEntry?, containsKey_eq_isSome_getEntry?, getEntry?_insertEntry]
   cases a == k <;> simp
 
-theorem containsKey_insertEntry_of_beq [BEq α] [PartialEquivBEq α] {l : List (Σ a, β a)} {k a : α} {v : β k} (h : a == k) :
+theorem containsKey_insertEntry_of_beq [BEq α] [PartialEquivBEq α] {l : List ((a : α) × β a)} {k a : α} {v : β k} (h : a == k) :
     containsKey a (insertEntry k v l) := by
   simp [h]
 
 @[simp]
-theorem containsKey_insertEntry_self [BEq α] [EquivBEq α] {l : List (Σ a, β a)} {k : α} {v : β k} :
+theorem containsKey_insertEntry_self [BEq α] [EquivBEq α] {l : List ((a : α) × β a)} {k : α} {v : β k} :
     containsKey k (insertEntry k v l) :=
   containsKey_insertEntry_of_beq BEq.refl
 
-theorem containsKey_of_containsKey_insertEntry [BEq α] [PartialEquivBEq α] {l : List (Σ a, β a)} {k a : α} {v : β k}
+theorem containsKey_of_containsKey_insertEntry [BEq α] [PartialEquivBEq α] {l : List ((a : α) × β a)} {k a : α} {v : β k}
     (h₁ : containsKey a (insertEntry k v l)) (h₂ : (a == k) = false) : containsKey a l := by
   rwa [containsKey_insertEntry, h₂, Bool.false_or] at h₁
 
-theorem getValueCast_insertEntry [BEq α] [LawfulBEq α] {l : List (Σ a, β a)} {k a : α} {v : β k} {h} :
+theorem getValueCast_insertEntry [BEq α] [LawfulBEq α] {l : List ((a : α) × β a)} {k a : α} {v : β k} {h} :
     getValueCast a (insertEntry k v l) h =
     if h' : a == k then
       cast (congrArg β (eq_of_beq h').symm) v
@@ -916,7 +916,7 @@ theorem getValueCast_insertEntry [BEq α] [LawfulBEq α] {l : List (Σ a, β a)}
   rw [← Option.some_inj, ← getValueCast?_eq_some_getValueCast, apply_dite Option.some, getValueCast?_insertEntry]
   simp only [← getValueCast?_eq_some_getValueCast]
 
-theorem getValueCast_insertEntry_self [BEq α] [LawfulBEq α] {l : List (Σ a, β a)} {k : α} {v : β k} :
+theorem getValueCast_insertEntry_self [BEq α] [LawfulBEq α] {l : List ((a : α) × β a)} {k : α} {v : β k} :
     getValueCast k (insertEntry k v l) containsKey_insertEntry_self = v := by
   simp [getValueCast_insertEntry]
 
@@ -929,32 +929,32 @@ theorem getValue_insertEntry_self {β : Type v} [BEq α] [EquivBEq α] {l : List
     getValue k (insertEntry k v l) containsKey_insertEntry_self = v := by
   simp [getValue_insertEntry]
 
-def insertEntryIfNew [BEq α] (k : α) (v : β k) (l : List (Σ a, β a)) : List (Σ a, β a) :=
+def insertEntryIfNew [BEq α] (k : α) (v : β k) (l : List ((a : α) × β a)) : List ((a : α) × β a) :=
   bif containsKey k l then l else ⟨k, v⟩ :: l
 
-theorem insertEntryIfNew_of_containsKey [BEq α] {l : List (Σ a, β a)} {k : α} {v : β k} (h : containsKey k l) :
+theorem insertEntryIfNew_of_containsKey [BEq α] {l : List ((a : α) × β a)} {k : α} {v : β k} (h : containsKey k l) :
     insertEntryIfNew k v l = l := by
   simp_all [insertEntryIfNew]
 
-theorem insertEntryIfNew_of_containsKey_eq_false [BEq α] {l : List (Σ a, β a)} {k : α} {v : β k} (h : containsKey k l = false) :
+theorem insertEntryIfNew_of_containsKey_eq_false [BEq α] {l : List ((a : α) × β a)} {k : α} {v : β k} (h : containsKey k l = false) :
     insertEntryIfNew k v l = ⟨k, v⟩ :: l := by
   simp_all [insertEntryIfNew]
 
 @[simp]
-theorem isEmpty_insertEntryIfNew [BEq α] {l : List (Σ a, β a)} {k : α} {v : β k} :
+theorem isEmpty_insertEntryIfNew [BEq α] {l : List ((a : α) × β a)} {k : α} {v : β k} :
     (insertEntryIfNew k v l).isEmpty = false := by
   cases h : containsKey k l
   · simp [insertEntryIfNew_of_containsKey_eq_false h]
   · rw [insertEntryIfNew_of_containsKey h]
     exact isEmpty_eq_false_of_containsKey h
 
-theorem getEntry?_insertEntryIfNew [BEq α] [PartialEquivBEq α] {l : List (Σ a, β a)} {k a : α} {v : β k} :
+theorem getEntry?_insertEntryIfNew [BEq α] [PartialEquivBEq α] {l : List ((a : α) × β a)} {k a : α} {v : β k} :
     getEntry? a (insertEntryIfNew k v l) = bif a == k && !containsKey k l then some ⟨k, v⟩ else getEntry? a l := by
   cases h : containsKey k l
   · simp [insertEntryIfNew_of_containsKey_eq_false h, getEntry?_cons]
   · simp [insertEntryIfNew_of_containsKey h]
 
-theorem getValueCast?_insertEntryIfNew [BEq α] [LawfulBEq α] {l : List (Σ a, β a)} {k a : α} {v : β k} :
+theorem getValueCast?_insertEntryIfNew [BEq α] [LawfulBEq α] {l : List ((a : α) × β a)} {k a : α} {v : β k} :
     getValueCast? a (insertEntryIfNew k v l) =
       if h : a == k ∧ containsKey k l = false then some (cast (congrArg β (eq_of_beq h.1).symm) v) else getValueCast? a l := by
   cases h : containsKey k l
@@ -966,7 +966,7 @@ theorem getValue?_insertEntryIfNew {β : Type v} [BEq α] [PartialEquivBEq α] {
     getValue? a (insertEntryIfNew k v l) = bif a == k && !containsKey k l then some v else getValue? a l := by
   simp [getValue?_eq_getEntry?, getEntry?_insertEntryIfNew, apply_bif (Option.map (fun (y : ((_ : α) × β)) => y.2))]
 
-theorem containsKey_insertEntryIfNew [BEq α] [PartialEquivBEq α] {l : List (Σ a, β a)} {k a : α} {v : β k} :
+theorem containsKey_insertEntryIfNew [BEq α] [PartialEquivBEq α] {l : List ((a : α) × β a)} {k a : α} {v : β k} :
     containsKey a (insertEntryIfNew k v l) = ((a == k) || containsKey a l) := by
   simp only [containsKey_eq_isSome_getEntry?, getEntry?_insertEntryIfNew, apply_bif Option.isSome,
     Option.isSome_some, Bool.cond_true_left]
@@ -974,11 +974,11 @@ theorem containsKey_insertEntryIfNew [BEq α] [PartialEquivBEq α] {l : List (Σ
   · simp
   · rw [Bool.true_and, Bool.true_or, getEntry?_congr h, Bool.not_or_self]
 
-theorem containsKey_insertEntryIfNew_self [BEq α] [EquivBEq α] {l : List (Σ a, β a)} {k : α}
+theorem containsKey_insertEntryIfNew_self [BEq α] [EquivBEq α] {l : List ((a : α) × β a)} {k : α}
     {v : β k} : containsKey k (insertEntryIfNew k v l) := by
   rw [containsKey_insertEntryIfNew, BEq.refl, Bool.true_or]
 
-theorem containsKey_of_containsKey_insertEntryIfNew [BEq α] [PartialEquivBEq α] {l : List (Σ a, β a)} {k a : α}
+theorem containsKey_of_containsKey_insertEntryIfNew [BEq α] [PartialEquivBEq α] {l : List ((a : α) × β a)} {k a : α}
     {v : β k} (h₁ : containsKey a (insertEntryIfNew k v l)) (h₂ : (a == k) = false) : containsKey a l := by
   rwa [containsKey_insertEntryIfNew, h₂, Bool.false_or] at h₁
 
@@ -986,14 +986,14 @@ theorem containsKey_of_containsKey_insertEntryIfNew [BEq α] [PartialEquivBEq α
 This is a restatement of `containsKey_insertEntryIfNew` that is written to exactly match the proof obligation in the
 statement of `getValueCast_insertEntryIfNew`.
 -/
-theorem containsKey_of_containsKey_insertEntryIfNew' [BEq α] [PartialEquivBEq α] {l : List (Σ a, β a)} {k a : α}
+theorem containsKey_of_containsKey_insertEntryIfNew' [BEq α] [PartialEquivBEq α] {l : List ((a : α) × β a)} {k a : α}
     {v : β k} (h₁ : containsKey a (insertEntryIfNew k v l)) (h₂ : ¬((a == k) ∧ containsKey k l = false)) : containsKey a l := by
   rw [Decidable.not_and_iff_or_not, Bool.not_eq_true, Bool.not_eq_false] at h₂
   rcases h₂ with h₂|h₂
   · rwa [containsKey_insertEntryIfNew, h₂, Bool.false_or] at h₁
   · rwa [insertEntryIfNew_of_containsKey h₂] at h₁
 
-theorem getValueCast_insertEntryIfNew [BEq α] [LawfulBEq α] {l : List (Σ a, β a)} {k a : α} {v : β k} {h} :
+theorem getValueCast_insertEntryIfNew [BEq α] [LawfulBEq α] {l : List ((a : α) × β a)} {k a : α} {v : β k} {h} :
     getValueCast a (insertEntryIfNew k v l) h =
     if h' : a == k ∧ containsKey k l = false then
       cast (congrArg β (eq_of_beq h'.1).symm) v
@@ -1009,7 +1009,7 @@ theorem getValue_insertEntryIfNew {β : Type v} [BEq α] [PartialEquivBEq α] {l
   rw [← Option.some_inj, ← getValue?_eq_some_getValue, apply_dite Option.some, getValue?_insertEntryIfNew, cond_eq_if, ← dite_eq_ite]
   simp [← getValue?_eq_some_getValue]
 
-theorem getValueCast!_insertEntryIfNew [BEq α] [LawfulBEq α] {l : List (Σ a, β a)} {k a : α} {v : β k} [Inhabited (β a)] :
+theorem getValueCast!_insertEntryIfNew [BEq α] [LawfulBEq α] {l : List ((a : α) × β a)} {k a : α} {v : β k} [Inhabited (β a)] :
     getValueCast! a (insertEntryIfNew k v l) =
       if h : a == k ∧ containsKey k l = false then cast (congrArg β (eq_of_beq h.1).symm) v else getValueCast! a l := by
   simp [getValueCast!_eq_getValueCast?, getValueCast?_insertEntryIfNew, apply_dite Option.get!]
@@ -1018,7 +1018,7 @@ theorem getValue!_insertEntryIfNew {β : Type v} [BEq α] [PartialEquivBEq α] [
     getValue! a (insertEntryIfNew k v l) = bif a == k && !containsKey k l then v else getValue! a l := by
   simp [getValue!_eq_getValue?, getValue?_insertEntryIfNew, apply_bif Option.get!]
 
-theorem getValueCastD_insertEntryIfNew [BEq α] [LawfulBEq α] {l : List (Σ a, β a)} {k a : α} {v : β k} {fallback : β a} :
+theorem getValueCastD_insertEntryIfNew [BEq α] [LawfulBEq α] {l : List ((a : α) × β a)} {k a : α} {v : β k} {fallback : β a} :
     getValueCastD a (insertEntryIfNew k v l) fallback =
       if h : a == k ∧ containsKey k l = false then cast (congrArg β (eq_of_beq h.1).symm) v else getValueCastD a l fallback := by
   simp [getValueCastD_eq_getValueCast?, getValueCast?_insertEntryIfNew, apply_dite (fun x => Option.getD x fallback)]
@@ -1028,11 +1028,11 @@ theorem getValueD_insertEntryIfNew {β : Type v} [BEq α] [PartialEquivBEq α] {
       bif a == k && !containsKey k l then v else getValueD a l fallback := by
   simp [getValueD_eq_getValue?, getValue?_insertEntryIfNew, apply_bif (fun x => Option.getD x fallback)]
 
-theorem length_insertEntryIfNew [BEq α] {l : List (Σ a, β a)} {k : α} {v : β k} :
+theorem length_insertEntryIfNew [BEq α] {l : List ((a : α) × β a)} {k : α} {v : β k} :
     (insertEntryIfNew k v l).length = bif containsKey k l then l.length else l.length + 1 := by
   simp [insertEntryIfNew, apply_bif List.length]
 
-theorem length_le_length_insertEntryIfNew [BEq α] {l : List (Σ a, β a)} {k : α} {v : β k} :
+theorem length_le_length_insertEntryIfNew [BEq α] {l : List ((a : α) × β a)} {k : α} {v : β k} :
     l.length ≤ (insertEntryIfNew k v l).length := by
   rw [length_insertEntryIfNew]
   cases containsKey k l
@@ -1040,7 +1040,7 @@ theorem length_le_length_insertEntryIfNew [BEq α] {l : List (Σ a, β a)} {k : 
   · simp
 
 @[simp]
-theorem keys_removeKey [BEq α] [PartialEquivBEq α] {l : List (Σ a, β a)} {k : α} :
+theorem keys_removeKey [BEq α] [PartialEquivBEq α] {l : List ((a : α) × β a)} {k : α} :
     keys (removeKey k l) = (keys l).erase k := by
   induction l using assoc_induction
   · rfl
@@ -1049,10 +1049,10 @@ theorem keys_removeKey [BEq α] [PartialEquivBEq α] {l : List (Σ a, β a)} {k 
     rw [BEq.comm]
     cases k' == k <;> simp [ih]
 
-theorem DistinctKeys.removeKey [BEq α] [PartialEquivBEq α] {l : List (Σ a, β a)} {k : α} : DistinctKeys l → DistinctKeys (removeKey k l) := by
+theorem DistinctKeys.removeKey [BEq α] [PartialEquivBEq α] {l : List ((a : α) × β a)} {k : α} : DistinctKeys l → DistinctKeys (removeKey k l) := by
   apply distinctKeys_of_sublist_keys (by simpa using erase_sublist _ _)
 
-theorem getEntry?_removeKey_self [BEq α] [PartialEquivBEq α] {l : List (Σ a, β a)} {k : α} (h : DistinctKeys l) :
+theorem getEntry?_removeKey_self [BEq α] [PartialEquivBEq α] {l : List ((a : α) × β a)} {k : α} (h : DistinctKeys l) :
     getEntry? k (removeKey k l) = none := by
   induction l using assoc_induction
   · simp
@@ -1064,11 +1064,11 @@ theorem getEntry?_removeKey_self [BEq α] [PartialEquivBEq α] {l : List (Σ a, 
         ← containsKey_eq_isSome_getEntry?, ← containsKey_congr (BEq.symm h')]
       exact h.containsKey_eq_false
 
-theorem getEntry?_removeKey_of_beq [BEq α] [PartialEquivBEq α] {l : List (Σ a, β a)} {k a : α} (hl : DistinctKeys l)
+theorem getEntry?_removeKey_of_beq [BEq α] [PartialEquivBEq α] {l : List ((a : α) × β a)} {k a : α} (hl : DistinctKeys l)
     (hka : a == k) : getEntry? a (removeKey k l) = none := by
   rw [← getEntry?_congr (BEq.symm hka), getEntry?_removeKey_self hl]
 
-theorem getEntry?_removeKey_of_false [BEq α] [PartialEquivBEq α] {l : List (Σ a, β a)} {k a : α}
+theorem getEntry?_removeKey_of_false [BEq α] [PartialEquivBEq α] {l : List ((a : α) × β a)} {k a : α}
     (hka : (a == k) = false) : getEntry? a (removeKey k l) = getEntry? a l := by
   induction l using assoc_induction
   · simp
@@ -1082,13 +1082,13 @@ theorem getEntry?_removeKey_of_false [BEq α] [PartialEquivBEq α] {l : List (Σ
       have hx : (a == k') = false := BEq.neq_of_neq_of_beq hka h'
       rw [getEntry?_cons_of_false hx]
 
-theorem getEntry?_removeKey [BEq α] [PartialEquivBEq α] {l : List (Σ a, β a)} {k a : α} (hl : DistinctKeys l) :
+theorem getEntry?_removeKey [BEq α] [PartialEquivBEq α] {l : List ((a : α) × β a)} {k a : α} (hl : DistinctKeys l) :
     getEntry? a (removeKey k l) = bif a == k then none else getEntry? a l := by
   cases h : a == k
   · simp [getEntry?_removeKey_of_false h, h]
   · simp [getEntry?_removeKey_of_beq hl h, h]
 
-theorem keys_filterMap [BEq α] {l : List (Σ a, β a)} {f : (a : α) → β a → Option (γ a)} :
+theorem keys_filterMap [BEq α] {l : List ((a : α) × β a)} {f : (a : α) → β a → Option (γ a)} :
     keys (l.filterMap fun p => (f p.1 p.2).map (⟨p.1, ·⟩)) = keys (l.filter fun p => (f p.1 p.2).isSome) := by
   induction l using assoc_induction
   · simp
@@ -1097,22 +1097,22 @@ theorem keys_filterMap [BEq α] {l : List (Σ a, β a)} {f : (a : α) → β a �
     cases f k v <;> simp [ih]
 
 @[simp]
-theorem keys_map [BEq α] {l : List (Σ a, β a)} {f : (a : α) → β a → γ a} :
+theorem keys_map [BEq α] {l : List ((a : α) × β a)} {f : (a : α) → β a → γ a} :
     keys (l.map fun p => ⟨p.1, f p.1 p.2⟩) = keys l := by
   induction l using assoc_induction <;> simp_all
 
-theorem DistinctKeys.filterMap [BEq α] [PartialEquivBEq α] {l : List (Σ a, β a)} {f : (a : α) → β a → Option (γ a)} :
+theorem DistinctKeys.filterMap [BEq α] [PartialEquivBEq α] {l : List ((a : α) × β a)} {f : (a : α) → β a → Option (γ a)} :
     DistinctKeys l → DistinctKeys (l.filterMap fun p => (f p.1 p.2).map (⟨p.1, ·⟩)) := by
   apply distinctKeys_of_sublist_keys
   rw [keys_filterMap, keys_eq_map, keys_eq_map]
   apply Sublist.map
   exact filter_sublist l
 
-theorem DistinctKeys.map [BEq α] {l : List (Σ a, β a)} {f : (a : α) → β a → γ a}
+theorem DistinctKeys.map [BEq α] {l : List ((a : α) × β a)} {f : (a : α) → β a → γ a}
     (h : DistinctKeys l) : DistinctKeys (l.map fun p => ⟨p.1, f p.1 p.2⟩) :=
   h.of_keys_eq keys_map.symm
 
-theorem DistinctKeys.filter [BEq α] {l : List (Σ a, β a)} {f : (a : α) → β a → Bool}
+theorem DistinctKeys.filter [BEq α] {l : List ((a : α) × β a)} {f : (a : α) → β a → Bool}
     (h : DistinctKeys l) : DistinctKeys (l.filter fun p => f p.1 p.2) :=
   distinctKeys_of_sublist (filter_sublist _) h
 
@@ -1138,23 +1138,23 @@ theorem getValue?_removeKey [BEq α] [PartialEquivBEq α] {l : List ((_ : α) ×
 
 end
 
-theorem containsKey_removeKey_self [BEq α] [PartialEquivBEq α] {l : List (Σ a, β a)} {k : α} (h : DistinctKeys l) :
+theorem containsKey_removeKey_self [BEq α] [PartialEquivBEq α] {l : List ((a : α) × β a)} {k : α} (h : DistinctKeys l) :
     containsKey k (removeKey k l) = false := by
   simp [containsKey_eq_isSome_getEntry?, getEntry?_removeKey_self h]
 
-theorem containsKey_removeKey_of_beq [BEq α] [PartialEquivBEq α] {l : List (Σ a, β a)} {k a : α} (hl : DistinctKeys l)
+theorem containsKey_removeKey_of_beq [BEq α] [PartialEquivBEq α] {l : List ((a : α) × β a)} {k a : α} (hl : DistinctKeys l)
     (hka : a == k) : containsKey a (removeKey k l) = false := by
   rw [containsKey_congr hka, containsKey_removeKey_self hl]
 
-theorem containsKey_removeKey_of_false [BEq α] [PartialEquivBEq α] {l : List (Σ a, β a)} {k a : α}
+theorem containsKey_removeKey_of_false [BEq α] [PartialEquivBEq α] {l : List ((a : α) × β a)} {k a : α}
     (hka : (a == k) = false) : containsKey a (removeKey k l) = containsKey a l := by
   simp [containsKey_eq_isSome_getEntry?, getEntry?_removeKey_of_false hka]
 
-theorem containsKey_removeKey [BEq α] [PartialEquivBEq α] {l : List (Σ a, β a)} {k a : α} (hl : DistinctKeys l) :
+theorem containsKey_removeKey [BEq α] [PartialEquivBEq α] {l : List ((a : α) × β a)} {k a : α} (hl : DistinctKeys l) :
     containsKey a (removeKey k l) = (!(a == k) && containsKey a l) := by
   simp [containsKey_eq_isSome_getEntry?, getEntry?_removeKey hl, apply_bif]
 
-theorem getValueCast?_removeKey [BEq α] [LawfulBEq α] {l : List (Σ a, β a)} {k a : α} (hl : DistinctKeys l) :
+theorem getValueCast?_removeKey [BEq α] [LawfulBEq α] {l : List ((a : α) × β a)} {k a : α} (hl : DistinctKeys l) :
     getValueCast? a (removeKey k l) = bif a == k then none else getValueCast? a l := by
   rw [getValueCast?_eq_getEntry?, Option.dmap_congr (getEntry?_removeKey hl)]
   rcases Bool.eq_false_or_eq_true (a == k) with h|h
@@ -1162,23 +1162,23 @@ theorem getValueCast?_removeKey [BEq α] [LawfulBEq α] {l : List (Σ a, β a)} 
   · rw [Option.dmap_congr (bif_neg h), getValueCast?_eq_getEntry?]
     exact (bif_neg h).symm
 
-theorem getValueCast?_removeKey_self [BEq α] [LawfulBEq α] {l : List (Σ a, β a)} {k : α} (hl : DistinctKeys l) :
+theorem getValueCast?_removeKey_self [BEq α] [LawfulBEq α] {l : List ((a : α) × β a)} {k : α} (hl : DistinctKeys l) :
     getValueCast? k (removeKey k l) = none := by
   rw [getValueCast?_removeKey hl, bif_pos BEq.refl]
 
-theorem getValueCast!_removeKey [BEq α] [LawfulBEq α] {l : List (Σ a, β a)} {k a : α} [Inhabited (β a)] (hl : DistinctKeys l) :
+theorem getValueCast!_removeKey [BEq α] [LawfulBEq α] {l : List ((a : α) × β a)} {k a : α} [Inhabited (β a)] (hl : DistinctKeys l) :
     getValueCast! a (removeKey k l) = bif a == k then default else getValueCast! a l := by
   simp [getValueCast!_eq_getValueCast?, getValueCast?_removeKey hl, apply_bif Option.get!]
 
-theorem getValueCast!_removeKey_self [BEq α] [LawfulBEq α] {l : List (Σ a, β a)} {k : α} [Inhabited (β k)] (hl : DistinctKeys l) :
+theorem getValueCast!_removeKey_self [BEq α] [LawfulBEq α] {l : List ((a : α) × β a)} {k : α} [Inhabited (β k)] (hl : DistinctKeys l) :
     getValueCast! k (removeKey k l) = default := by
   simp [getValueCast!_eq_getValueCast?, getValueCast?_removeKey_self hl]
 
-theorem getValueCastD_removeKey [BEq α] [LawfulBEq α] {l : List (Σ a, β a)} {k a : α} {fallback : β a} (hl : DistinctKeys l) :
+theorem getValueCastD_removeKey [BEq α] [LawfulBEq α] {l : List ((a : α) × β a)} {k a : α} {fallback : β a} (hl : DistinctKeys l) :
     getValueCastD a (removeKey k l) fallback = bif a == k then fallback else getValueCastD a l fallback := by
   simp [getValueCastD_eq_getValueCast?, getValueCast?_removeKey hl, apply_bif (fun x => Option.getD x fallback)]
 
-theorem getValueCastD_removeKey_self [BEq α] [LawfulBEq α] {l : List (Σ a, β a)} {k : α} {fallback : β k} (hl : DistinctKeys l) :
+theorem getValueCastD_removeKey_self [BEq α] [LawfulBEq α] {l : List ((a : α) × β a)} {k : α} {fallback : β k} (hl : DistinctKeys l) :
     getValueCastD k (removeKey k l) fallback = fallback := by
   simp [getValueCastD_eq_getValueCast?, getValueCast?_removeKey_self hl]
 
@@ -1198,11 +1198,11 @@ theorem getValueD_removeKey_self {β : Type v} [BEq α] [PartialEquivBEq α] {l 
     (hl : DistinctKeys l) : getValueD k (removeKey k l) fallback = fallback := by
   simp [getValueD_eq_getValue?, getValue?_removeKey_self hl]
 
-theorem containsKey_of_containsKey_removeKey [BEq α] [PartialEquivBEq α] {l : List (Σ a, β a)} {k a : α} (hl : DistinctKeys l) :
+theorem containsKey_of_containsKey_removeKey [BEq α] [PartialEquivBEq α] {l : List ((a : α) × β a)} {k a : α} (hl : DistinctKeys l) :
     containsKey a (removeKey k l) → containsKey a l := by
   simp [containsKey_removeKey hl]
 
-theorem getValueCast_removeKey [BEq α] [LawfulBEq α] {l : List (Σ a, β a)} {k a : α} {h} (hl : DistinctKeys l) :
+theorem getValueCast_removeKey [BEq α] [LawfulBEq α] {l : List ((a : α) × β a)} {k a : α} {h} (hl : DistinctKeys l) :
     getValueCast a (removeKey k l) h = getValueCast a l (containsKey_of_containsKey_removeKey hl h) := by
   rw [containsKey_removeKey hl, Bool.and_eq_true, Bool.not_eq_true'] at h
   rw [← Option.some_inj, ← getValueCast?_eq_some_getValueCast, getValueCast?_removeKey hl, h.1, cond_false,
@@ -1213,7 +1213,7 @@ theorem getValue_removeKey {β : Type v} [BEq α] [PartialEquivBEq α] {l : List
   rw [containsKey_removeKey hl, Bool.and_eq_true, Bool.not_eq_true'] at h
   rw [← Option.some_inj, ← getValue?_eq_some_getValue, getValue?_removeKey hl, h.1, cond_false, ← getValue?_eq_some_getValue]
 
-theorem getEntry?_of_perm [BEq α] [PartialEquivBEq α] {l l' : List (Σ a, β a)} {a : α} (hl : DistinctKeys l)
+theorem getEntry?_of_perm [BEq α] [PartialEquivBEq α] {l l' : List ((a : α) × β a)} {a : α} (hl : DistinctKeys l)
     (h : Perm l l') : getEntry? a l = getEntry? a l' := by
   induction h
   · simp
@@ -1229,7 +1229,7 @@ theorem getEntry?_of_perm [BEq α] [PartialEquivBEq α] {l l' : List (Σ a, β a
     exact ((Bool.eq_false_iff.1 hl.2.1).elim (BEq.trans (BEq.symm h₁) h₂)).elim
   · next l₁ l₂ l₃ hl₁₂ _ ih₁ ih₂ => exact (ih₁ hl).trans (ih₂ (hl.perm (hl₁₂.symm)))
 
-theorem containsKey_of_perm [BEq α] [PartialEquivBEq α] {l l' : List (Σ a, β a)} {k : α}
+theorem containsKey_of_perm [BEq α] [PartialEquivBEq α] {l l' : List ((a : α) × β a)} {k : α}
     (h : Perm l l') : containsKey k l = containsKey k l' := by
   induction h
   · simp
@@ -1239,20 +1239,20 @@ theorem containsKey_of_perm [BEq α] [PartialEquivBEq α] {l l' : List (Σ a, β
     simp only [← Bool.or_assoc, Bool.or_comm]
   · next _ _ _ _ _ ih₁ ih₂ => exact ih₁.trans ih₂
 
-theorem getValueCast?_of_perm [BEq α] [LawfulBEq α] {l l' : List (Σ a, β a)} {a : α} (hl : DistinctKeys l)
+theorem getValueCast?_of_perm [BEq α] [LawfulBEq α] {l l' : List ((a : α) × β a)} {a : α} (hl : DistinctKeys l)
     (h : Perm l l') : getValueCast? a l = getValueCast? a l' := by
   rw [getValueCast?_eq_getEntry?, getValueCast?_eq_getEntry?, Option.dmap_congr (getEntry?_of_perm hl h)]
 
-theorem getValueCast_of_perm [BEq α] [LawfulBEq α] {l l' : List (Σ a, β a)} {a : α} {h'} (hl : DistinctKeys l)
+theorem getValueCast_of_perm [BEq α] [LawfulBEq α] {l l' : List ((a : α) × β a)} {a : α} {h'} (hl : DistinctKeys l)
     (h : Perm l l') : getValueCast a l h' = getValueCast a l' ((containsKey_of_perm h).symm.trans h') := by
   rw [← Option.some_inj, ← getValueCast?_eq_some_getValueCast, ← getValueCast?_eq_some_getValueCast,
     getValueCast?_of_perm hl h]
 
-theorem getValueCast!_of_perm [BEq α] [LawfulBEq α] {l l' : List (Σ a, β a)} {a : α} [Inhabited (β a)] (hl : DistinctKeys l)
+theorem getValueCast!_of_perm [BEq α] [LawfulBEq α] {l l' : List ((a : α) × β a)} {a : α} [Inhabited (β a)] (hl : DistinctKeys l)
     (h : Perm l l') : getValueCast! a l = getValueCast! a l' := by
   simp only [getValueCast!_eq_getValueCast?, getValueCast?_of_perm hl h]
 
-theorem getValueCastD_of_perm [BEq α] [LawfulBEq α] {l l' : List (Σ a, β a)} {a : α} {fallback : β a} (hl : DistinctKeys l)
+theorem getValueCastD_of_perm [BEq α] [LawfulBEq α] {l l' : List ((a : α) × β a)} {a : α} {fallback : β a} (hl : DistinctKeys l)
     (h : Perm l l') : getValueCastD a l fallback = getValueCastD a l' fallback := by
   simp only [getValueCastD_eq_getValueCast?, getValueCast?_of_perm hl h]
 
@@ -1278,7 +1278,7 @@ theorem getValueD_of_perm [BEq α] [PartialEquivBEq α] {l l' : List ((_ : α) �
 
 end
 
-theorem perm_cons_getEntry [BEq α] {l : List (Σ a, β a)} {a : α} (h : containsKey a l) :
+theorem perm_cons_getEntry [BEq α] {l : List ((a : α) × β a)} {a : α} (h : containsKey a l) :
     ∃ l', Perm l (getEntry a l h :: l') := by
   induction l using assoc_induction
   · simp at h
@@ -1291,7 +1291,7 @@ theorem perm_cons_getEntry [BEq α] {l : List (Σ a, β a)} {a : α} (h : contai
     · exact ⟨t, by rw [getEntry_cons_of_beq hk]; exact Perm.refl _⟩
 
 -- Note: this theorem becomes false if you don't assume that BEq is reflexive on α.
-theorem getEntry?_ext [BEq α] [EquivBEq α] {l l' : List (Σ a, β a)} (hl : DistinctKeys l) (hl' : DistinctKeys l')
+theorem getEntry?_ext [BEq α] [EquivBEq α] {l l' : List ((a : α) × β a)} (hl : DistinctKeys l) (hl' : DistinctKeys l')
     (h : ∀ a, getEntry? a l = getEntry? a l') : Perm l l' := by
   induction l using assoc_induction generalizing l'
   · induction l' using assoc_induction
@@ -1311,38 +1311,38 @@ theorem getEntry?_ext [BEq α] [EquivBEq α] {l l' : List (Σ a, β a)} (hl : Di
     · rw [getEntry?_congr hk', getEntry?_congr hk', getEntry?_eq_none.2 hl.containsKey_eq_false,
           getEntry?_eq_none.2 (hl'.perm hl''.symm).containsKey_eq_false]
 
-theorem replaceEntry_of_perm [BEq α] [EquivBEq α] {l l' : List (Σ a, β a)} {k : α} {v : β k}
+theorem replaceEntry_of_perm [BEq α] [EquivBEq α] {l l' : List ((a : α) × β a)} {k : α} {v : β k}
     (hl : DistinctKeys l) (h : Perm l l') : Perm (replaceEntry k v l) (replaceEntry k v l') := by
   apply getEntry?_ext hl.replaceEntry (hl.perm h.symm).replaceEntry
   simp [getEntry?_replaceEntry, getEntry?_of_perm hl h, containsKey_of_perm h]
 
-theorem insertEntry_of_perm [BEq α] [EquivBEq α] {l l' : List (Σ a, β a)} {k : α} {v : β k}
+theorem insertEntry_of_perm [BEq α] [EquivBEq α] {l l' : List ((a : α) × β a)} {k : α} {v : β k}
     (hl : DistinctKeys l) (h : Perm l l') : Perm (insertEntry k v l) (insertEntry k v l') := by
   apply getEntry?_ext hl.insertEntry (hl.perm h.symm).insertEntry
   simp [getEntry?_insertEntry, getEntry?_of_perm hl h]
 
-theorem removeKey_of_perm [BEq α] [EquivBEq α] {l l' : List (Σ a, β a)} {k : α}
+theorem removeKey_of_perm [BEq α] [EquivBEq α] {l l' : List ((a : α) × β a)} {k : α}
     (hl : DistinctKeys l) (h : Perm l l') : Perm (removeKey k l) (removeKey k l') := by
   apply getEntry?_ext hl.removeKey (hl.perm h.symm).removeKey
   simp [getEntry?_removeKey hl, getEntry?_removeKey (hl.perm h.symm), getEntry?_of_perm hl h]
 
 @[simp]
-theorem getEntry?_append [BEq α] {l l' : List (Σ a, β a)} {a : α} :
+theorem getEntry?_append [BEq α] {l l' : List ((a : α) × β a)} {a : α} :
     getEntry? a (l ++ l') = (getEntry? a l).or (getEntry? a l') := by
   induction l using assoc_induction
   · simp
   · next k' v' t ih => cases h : a == k' <;> simp_all [getEntry?_cons]
 
-theorem getEntry?_append_of_containsKey_eq_false [BEq α] {l l' : List (Σ a, β a)} {a : α}
+theorem getEntry?_append_of_containsKey_eq_false [BEq α] {l l' : List ((a : α) × β a)} {a : α}
     (h : containsKey a l' = false) : getEntry? a (l ++ l') = getEntry? a l := by
   rw [getEntry?_append, getEntry?_eq_none.2 h, Option.or_none]
 
 @[simp]
-theorem containsKey_append [BEq α] {l l' : List (Σ a, β a)} {a : α} :
+theorem containsKey_append [BEq α] {l l' : List ((a : α) × β a)} {a : α} :
     containsKey a (l ++ l') = (containsKey a l || containsKey a l') := by
   simp [containsKey_eq_isSome_getEntry?]
 
-theorem containsKey_bind_eq_false [BEq α] {γ : Type w} {l : List γ} {f : γ → List (Σ a, β a)} {a : α}
+theorem containsKey_bind_eq_false [BEq α] {γ : Type w} {l : List γ} {f : γ → List ((a : α) × β a)} {a : α}
     (h : ∀ (i : Nat) (h : i < l.length), containsKey a (f l[i]) = false) : containsKey a (l.bind f) = false := by
   induction l
   · simp
@@ -1354,7 +1354,7 @@ theorem containsKey_bind_eq_false [BEq α] {γ : Type w} {l : List γ} {f : γ �
       intro i hi
       simpa using h (i + 1) (by simp only [List.length_cons]; omega)
 
-theorem containsKey_append_of_not_contains_right [BEq α] {l l' : List (Σ a, β a)} {a : α}
+theorem containsKey_append_of_not_contains_right [BEq α] {l l' : List ((a : α) × β a)} {a : α}
     (hl' : containsKey a l' = false) : containsKey a (l ++ l') = containsKey a l := by
   simp [hl']
 
@@ -1371,18 +1371,18 @@ theorem getValue_append_of_containsKey_eq_false {β : Type v} [BEq α] {l l' : L
     (h : containsKey a l' = false) : getValue a (l ++ l') h' = getValue a l ((containsKey_append_of_not_contains_right h).symm.trans h') := by
   rw [← Option.some_inj, ← getValue?_eq_some_getValue, ← getValue?_eq_some_getValue, getValue?_append_of_containsKey_eq_false h]
 
-theorem getValueCast?_append_of_containsKey_eq_false [BEq α] [LawfulBEq α] {l l' : List (Σ a, β a)} {a : α}
+theorem getValueCast?_append_of_containsKey_eq_false [BEq α] [LawfulBEq α] {l l' : List ((a : α) × β a)} {a : α}
     (hl' : containsKey a l' = false) : getValueCast? a (l ++ l') = getValueCast? a l := by
   rw [getValueCast?_eq_getEntry?, getValueCast?_eq_getEntry?, Option.dmap_congr getEntry?_append,
     Option.dmap_congr (by rw [getEntry?_eq_none.2 hl']), Option.dmap_congr (by rw [Option.or_none])]
 
-theorem getValueCast_append_of_containsKey_eq_false [BEq α] [LawfulBEq α] {l l' : List (Σ a, β a)} {a : α} {h}
+theorem getValueCast_append_of_containsKey_eq_false [BEq α] [LawfulBEq α] {l l' : List ((a : α) × β a)} {a : α} {h}
     (hl' : containsKey a l' = false) :
     getValueCast a (l ++ l') h = getValueCast a l ((containsKey_append_of_not_contains_right hl').symm.trans h) := by
   rw [← Option.some_inj, ← getValueCast?_eq_some_getValueCast, ← getValueCast?_eq_some_getValueCast,
     getValueCast?_append_of_containsKey_eq_false hl']
 
-theorem replaceEntry_append_of_containsKey_left [BEq α] {l l' : List (Σ a, β a)} {k : α}
+theorem replaceEntry_append_of_containsKey_left [BEq α] {l l' : List ((a : α) × β a)} {k : α}
     {v : β k} (h : containsKey k l) : replaceEntry k v (l ++ l') = replaceEntry k v l ++ l' := by
   induction l using assoc_induction
   · simp at h
@@ -1392,7 +1392,7 @@ theorem replaceEntry_append_of_containsKey_left [BEq α] {l l' : List (Σ a, β 
     · simpa [replaceEntry_cons, h'] using ih (h.resolve_left (Bool.not_eq_true _ ▸ h'))
     · simp [replaceEntry_cons, h']
 
-theorem replaceEntry_append_of_containsKey_left_eq_false [BEq α] {l l' : List (Σ a, β a)} {k : α}
+theorem replaceEntry_append_of_containsKey_left_eq_false [BEq α] {l l' : List ((a : α) × β a)} {k : α}
     {v : β k} (h : containsKey k l = false) : replaceEntry k v (l ++ l') = l ++ replaceEntry k v l' := by
   induction l using assoc_induction
   · simp
@@ -1400,21 +1400,21 @@ theorem replaceEntry_append_of_containsKey_left_eq_false [BEq α] {l l' : List (
     simp only [containsKey_cons, Bool.or_eq_false_iff] at h
     simpa [replaceEntry_cons, h.1] using ih h.2
 
-theorem replaceEntry_append_of_containsKey_right_eq_false [BEq α] {l l' : List (Σ a, β a)} {k : α}
+theorem replaceEntry_append_of_containsKey_right_eq_false [BEq α] {l l' : List ((a : α) × β a)} {k : α}
     {v : β k} (h : containsKey k l' = false) : replaceEntry k v (l ++ l') = replaceEntry k v l ++ l' := by
   cases h' : containsKey k l
   · rw [replaceEntry_of_containsKey_eq_false, replaceEntry_of_containsKey_eq_false h']
     simpa using ⟨h', h⟩
   · rw [replaceEntry_append_of_containsKey_left h']
 
-theorem insertEntry_append_of_not_contains_right [BEq α] {l l' : List (Σ a, β a)}
+theorem insertEntry_append_of_not_contains_right [BEq α] {l l' : List ((a : α) × β a)}
     {k : α} {v : β k} (h' : containsKey k l' = false) :
     insertEntry k v (l ++ l') = insertEntry k v l ++ l' := by
   cases h : containsKey k l
   · simp [insertEntry, containsKey_append, h, h']
   · simp [insertEntry, containsKey_append, h, h', replaceEntry_append_of_containsKey_left h]
 
-theorem removeKey_append_of_containsKey_right_eq_false [BEq α] {l l' : List (Σ a, β a)} {k : α}
+theorem removeKey_append_of_containsKey_right_eq_false [BEq α] {l l' : List ((a : α) × β a)} {k : α}
     (h : containsKey k l' = false) : removeKey k (l ++ l') = removeKey k l ++ l' := by
   induction l using assoc_induction
   · simp [removeKey_of_containsKey_eq_false h]
