src/Std/Data/DHashMap/Internal/List/HashesTo.lean
@@ -21,10 +21,10 @@ variable {α : Type u} {β : α → Type v}
 
 @[simp]
 theorem hashesTo_nil [BEq α] [Hashable α] {i : Nat} {size : Nat} :
-    HashesTo ([] : List (Σ a, β a)) i size where
+    HashesTo ([] : List ((a : α) × β a)) i size where
   hash_self := by simp
 
-theorem hashesTo_cons [BEq α] [Hashable α] {i : Nat} {size : Nat} {l : List (Σ a, β a)} {k : α}
+theorem hashesTo_cons [BEq α] [Hashable α] {i : Nat} {size : Nat} {l : List ((a : α) × β a)} {k : α}
     {v : β k} (h : (h' : 0 < size) → (mkIdx size h' (hash k)).1.toNat = i) :
     HashesTo l i size → HashesTo (⟨k, v⟩ :: l) i size := by
   refine fun ⟨ih⟩ => ⟨fun h' k' hk => ?_⟩
@@ -33,7 +33,7 @@ theorem hashesTo_cons [BEq α] [Hashable α] {i : Nat} {size : Nat} {l : List (�
   · exact h h'
   · exact ih h' _ hk
 
-theorem HashesTo.containsKey_eq_false [BEq α] [Hashable α] [LawfulHashable α] {l : List (Σ a, β a)} {i : Nat} {size : Nat} (hs : 0 < size)
+theorem HashesTo.containsKey_eq_false [BEq α] [Hashable α] [LawfulHashable α] {l : List ((a : α) × β a)} {i : Nat} {size : Nat} (hs : 0 < size)
     (h : HashesTo l i size) (k : α) : (mkIdx size hs (hash k)).1.toNat ≠ i → containsKey k l = false := by
   rw [← Decidable.not_imp_not]
   simp only [Bool.not_eq_false, containsKey_eq_true_iff_exists_mem]
